Advanced proof to P2b and P2c point

Distributed/paxos_model.lean
@@ -5,7 +5,7 @@ open Model
 
 -- Type to represent the values chosen by the algorithm
 def Value := Nat
-deriving OfNat, BEq, DecidableEq, Ord, LT
+deriving OfNat, BEq, DecidableEq, Ord, LT, LE
 
 -- Type to represent the Id for the proposals issued by the proposers
 
@@ -15,7 +15,7 @@ deriving OfNat, BEq, DecidableEq, Ord, LT, HAdd, HMul, HMod, LE
 -- Type to represent the messages sent by the values
 inductive Message where
 | Prepare (propId: PropId) : Message
-| Promise (propId: PropId) (acceptId: Nat) (propVal: (Option Value) × PropId): Message
+| Promise (propId: PropId) (acceptId: Nat) (propVal: Option (Value × PropId)): Message
 | Accept (a: PropId × Value): Message
 | Learn (v: Fin a × Value × PropId )
 
@@ -64,10 +64,6 @@ inductive FailureStep: System a l p -> System a l p -> Prop where
 | lostmessage : ∀ (s1: System a l p) m n2, MessageIsLost m s1.network n2
 -> FailureStep s1 {s1 with network := n2}
 
-
-
-
-
 -- Algorithm steps
 @[simp]
 -- A proposer sends a proposal in the network with a new Id
@@ -76,31 +72,32 @@ m = Message.Prepare (uniqueId p1)  ∧ n2.messages = m :: n1.messages ∧ p2 = {
 
 @[simp]
 def AcceptorReceivesPrepare (n: PropId) (a1 a2: Acceptor a) (n1 n2: Network) (m: Message) :=
-   (m ∈ n1.messages ∧ m = Message.Prepare n ∧ n > a1.maxPrepareId) ∧ a2 = {a1 with maxPrepareId := n} ∧ n2.messages = (Message.Promise n a1.id (a1.maxProp, a1.maxPrepareId)) :: n1.messages
+   (m ∈ n1.messages ∧ m = Message.Prepare n ∧ n > a1.maxPrepareId) ∧ a2 = {a1 with maxPrepareId := n} ∧ n2.messages = (Message.Promise n a1.id a1.accepted) :: n1.messages
 
 @[simp]
-def ProposerReceivesPromise (maxP: Nat) (accId: Fin a) (maxV: Option Value) (p1 p2: Proposer p a) (n: Network) (m: Message) :=
-    m = Message.Promise p1.propId accId (maxV, maxP) ∧  m ∈ n.messages ∧ 
-    if (maxP > p1.accPropId && maxV != none)
-    then  p2 = {p1 with propRec := insertElem p1.propRec accId, accPropId := maxP, propVal := maxV}
+def ProposerReceivesPromise (maxP: Nat) (accId: Fin a) (p1 p2: Proposer p a) (n: Network) (m: Message) :=
+    ∀ opt v id,
+    m = Message.Promise p1.propId accId opt ∧  m ∈ n.messages ∧ 
+    if (maxP > p1.accPropId && opt == some (v, id))
+    then  p2 = {p1 with propRec := insertElem p1.propRec accId, accPropId := id, propVal := v}
     else p2 = {p1 with propRec := insertElem p1.propRec accId}
 
 @[simp]
-def ProposerSendsAcceptor (v: Value) (p: Proposer p a) (n1 n2: Network) :=
-    count p.propRec > (a / 2) ∧
-    if p.propVal == some v then
-       n2.messages = (Message.Accept (p.propId, v)) :: n1.messages
+def ProposerSendsAcceptor (v: Value) (p1 p2: Proposer p a) (n1 n2: Network) :=
+    count p1.propRec > (a / 2) ∧ p2 = {p1 with propVal := v} ∧ 
+    if p1.propVal == some v then
+       n2.messages = (Message.Accept (p1.propId, v)) :: n1.messages
     else
-       n2.messages = (Message.Accept (p.propId, v)) :: n1.messages 
+       n2.messages = (Message.Accept (p1.propId, v)) :: n1.messages 
     
 @[simp]
-def AcceptorAccepts (id: PropId) (v: Value) (a1 a2: Acceptor a) (m: Message) :=
-    m = Message.Accept (id, v) ∧ a1.maxPrepareId < id 
-    ∧ a2 = {a1 with accepted := some (id, v)}
+def AcceptorAccepts (id: PropId) (v: Value) (a1 a2: Acceptor a) (n: Network) (m: Message) :=
+    m = Message.Accept (id, v) ∧ a1.maxPrepareId <= id ∧ m ∈ n.messages
+    ∧ a2 = {a1 with accepted := some (v, id),  maxPrepareId := id}
 
 @[simp]
 def SendLearner (acc: Acceptor a) (n1 n2: Network) (v: Value) (id: PropId) :=
-    acc.accepted = some (id, v) ∧ 
+    acc.accepted = some (v, id) ∧ 
     n2.messages = (Message.Learn (acc.id, v, id)) :: n1.messages
 
 @[simp]
@@ -116,10 +113,10 @@ def ChooseVal (l1 l2: Learner a l) (v: Value) (id: PropId):=
 
 inductive WorkingStep {a l p: Nat}: System a l p -> System a l p -> Prop where
 | sendprepare: ∀ s n2 m i p2, ProposerSendsPrepare (s.proposers i) p2 s.network n2 m -> WorkingStep s {s with proposers := updateMap s.proposers i p2, network := n2}
-| sendpromise: ∀ s i n m a2 n2, AcceptorReceivesPrepare n (s.acceptors i) a2 s.network n2 m -> WorkingStep s {s with network := n2}
-| receivepromise: ∀ i s maxN accId maxV p2 m, ProposerReceivesPromise maxN accId maxV (s.proposers i) p2 s.network m -> WorkingStep s {s with proposers := updateMap s.proposers i p2}
-| sendacceptor : ∀ s v n2 i, ProposerSendsAcceptor v (s.proposers i) s.network n2 -> WorkingStep s {s with network := n2}
-| receiveacceptor: ∀ id s i v a2 m, AcceptorAccepts id v (s.acceptors i) a2 m -> WorkingStep s {s with acceptors := updateMap s.acceptors i a2}
+| sendpromise: ∀ s i n m a2 n2, AcceptorReceivesPrepare n (s.acceptors i) a2 s.network n2 m -> WorkingStep s {s with network := n2,  acceptors := updateMap s.acceptors i a2}
+| receivepromise: ∀ i s maxN accId p2 m, ProposerReceivesPromise maxN accId (s.proposers i)  p2 s.network m -> WorkingStep s {s with proposers := updateMap s.proposers i p2}
+| sendacceptor : ∀ s v n2 i, ProposerSendsAcceptor v (s.proposers i) p2 s.network n2 -> WorkingStep s {s with network := n2, proposers := updateMap s.proposers i p2}
+| receiveacceptor: ∀ id s i v a2 m, AcceptorAccepts id v (s.acceptors i) a2 s.network m -> WorkingStep s {s with acceptors := updateMap s.acceptors i a2}
 | sendlearner: ∀ s i n2 v id, SendLearner (s.acceptors i) s.network n2 v id -> WorkingStep s {s with network := n2}
 | receivelearner: ∀ s i l2 m v id acc, RecvLearner (s.network) (s.learners i) l2 m v acc id -> WorkingStep s {s with learners := updateMap s.learners i l2}
 | choosefinalvalue: ∀ l2 v i id, ChooseVal (s.learners i) l2 v id -> WorkingStep s  {s with learners := updateMap s.learners i l2}
