Distributed/paxos_proof_simp.lean
@@ -1,0 +1,533 @@
+import Distributed.base_structures
+import Distributed.paxos_model
+import Mathlib.Tactic.ByContra
+import Mathlib.Tactic.Cases 
+
+open Model
+open PaxosModel
+namespace PaxosProof
+
+theorem idIsK (s1: System a l p):
+systemIsValid s1
+-> ∀ k, (s1.acceptors k).id = k := by
+intros svalid; rcases  svalid with ⟨ s0, s0Inits, s0Steps ⟩
+induction s0Steps
+. simp [systemInits, acceptorInits] at s0Inits; simp [s0Inits]
+. rename_i s2 s3 steps step IH;
+  cases step <;> rename_i stepRule <;> cases stepRule <;> try (rename_i stepRule; simp at stepRule; grind)
+  intros k; simp [updateMap] at *; split <;> try grind
+  intros k; simp [updateMap] at *; split <;> try grind
+  
+def acc_invariant (s1 : System a l p) (v : Value) (id: PropId):=
+  ∃ (s : Set a), count s > a / 2 ∧
+    (∀ i, contains s i →
+      ∃ id', id' >= id ∧ (s1.acceptors i).accepted = some (v, id'))
+
+def mess_invariant (s1 : System a l p) (v : Value) (id: PropId) :=
+  ∃ (s : Set a), count s > a / 2 ∧
+    (∀ i, contains s i →
+      Message.Learn (i, v, id) ∈ s1.network.messages)
+
+def learn_invariant (s1 : System a l p) (v : Value) (j: Fin l) (id: PropId):=
+   ∃ (s : Set a), count s > a / 2 ∧
+    ∀ i, contains s i →
+      (s1.learners j).decMap i = some (v, id)
+
+def inv2 (s1: System a l p) (j: Fin l) (i: Fin a) (v: Value) (id: PropId):=
+(s1.learners j).decMap i = some (v, id)
+->  Message.Learn (i, v, id) ∈ s1.network.messages
+
+
+def inv3 (s1: System a l p) (i: Fin a) (v: Value) (id: PropId):=
+Message.Learn (i, v, id) ∈ s1.network.messages
+->  Message.Accept (id, v) ∈ s1.network.messages
+
+
+def inv31 (s1: System a l p) (i: Fin a) (v: Value) (id: PropId):=
+(s1.acceptors i).accepted = some (v, id)
+->  Message.Accept (id, v) ∈ s1.network.messages
+
+
+def inv4b1 (s: System a l p) (v1 v2 : Value) (id: PropId) :=
+Message.Accept (id, v1) ∈ s.network.messages
+-> Message.Accept (id, v2) ∈ s.network.messages
+-> v1 = v2
+
+def inv4b (s: System a l p) (v : Value) (id: PropId) :=
+(∃ set, count set > a / 2 ∧ (∀ (i: Fin a), contains  set i -> Message.Learn (i, v, id) ∈ s.network.messages))
+-> ∀ id' v', Message.Accept (id', v') ∈ s.network.messages
+->  id' >= id
+->  v = v'
+
+
+def inv4c (s: System a l p) (v : Value) (id: PropId) :=
+Message.Accept (id, v) ∈ s.network.messages
+-> (∃ set, count set > a / 2 ∧ ((∀ (i: Fin a), contains  set i ->
+(¬(∃ id' v', (s.acceptors i).accepted = some (v', id') ∧ id' < id)))
+∨ (∀ (i: Fin a), contains  set i ->
+(∃ idmax, idmax < id  ∧
+(∃ i, contains set i = true ∧ (s.acceptors i).accepted  = some (v, idmax))
+∧ 
+(∀ i, contains set i = true ->
+∀ v' id', (s.acceptors i).accepted = some (v', id')
+-> id' <= idmax)
+))))
+
+
+
+
+def inv42 (s1: System a l p) (i: Fin a) (v: Value) (id: PropId):=
+Message.Learn (i, v, id) ∈ s1.network.messages
+-> (s1.acceptors i).maxPrepareId >= id
+
+
+def inv43 (s1: System a l p) (i: Fin a) (v: Value) (id: PropId):=
+(s1.acceptors i).accepted = some (v, id)
+-> (s1.acceptors i).maxPrepareId >= id
+
+def inv4a1 (s: System a l p) (i: Fin a) (v : Value) (id: PropId) :=
+(s.acceptors i).accepted = some (v, id)
+-> Message.Accept (id, v) ∈ s.network.messages
+
+def inv4a (s: System a l p) (v : Value) (id: PropId) :=
+(∃ set, count set > a / 2 ∧ (∀ (i: Fin a), contains  set i -> Message.Learn (i, v, id) ∈ s.network.messages))
+-> ∀ id' i v', (s.acceptors i).accepted = some (v', id')
+->  id' >= id
+->  v = v'
+
+
+def inv41 (s1: System a l p) (i: Fin a) (v: Value) (id: PropId):=
+Message.Learn (i, v, id) ∈ s1.network.messages
+-> ∃ v' id', id' >= id ∧ (s1.acceptors i).accepted = some (v', id')
+
+def inv4 (s: System a l p) (v: Value) (id: PropId) :=
+(∃ set, count set > a / 2 ∧ (∀ (i: Fin a), contains  set i -> Message.Learn (i, v, id) ∈ s.network.messages))
+-> ∃ id', id' >= id ∧ acc_invariant s v id'
+
+
+
+
+
+
+
+theorem inv43Proof_ind (s1 s2: System a l p) (i: Fin a)  (v: Value) (id: PropId) :
+step s1 s2
+-> inv43 s1 i v id
+-> (∀ i, (s1.acceptors i).id = i)
+-> inv43 s2 i v id := by
+simp [inv43]; intros step IH kIsTrue learnInN
+cases step <;> rename_i stepRule <;> cases stepRule <;> (try (rename_i stepRule; simp at stepRule; grind)) <;> (try (simp [updateMap] at *; split <;> try grind  ))
+. rename_i j pid mess acc net stepRule eq; subst eq
+  split at learnInN <;> try grind
+  rcases stepRule with ⟨ messRules, accNat, netNat⟩; subst accNat 
+  simp at ⊢ learnInN; have b1 := IH learnInN; have b2 := messRules.right.right
+  exact Nat.le_of_lt (Nat.lt_of_le_of_lt b1 b2)
+. rename_i stepRule eq; split at learnInN <;> try grind
+  rcases stepRule with ⟨ messAcc, b2, mInN, accNat⟩; subst eq; subst accNat
+  simp at ⊢ learnInN; simp [learnInN, PropId]
+  
+
+
+theorem inv43Proof (s: System a l p) (v: Value) (i: Fin a) (id: PropId)  :
+systemIsValid s
+-> inv43 s i v id:= by
+intros sIsValid
+have ⟨ s0, s0Inits, s0Steps ⟩ := sIsValid
+induction s0Steps  with
+| refl =>
+  simp [systemInits, acceptorInits] at s0Inits
+  simp [inv43, s0Inits] at ⊢
+| trans s2 s3 s0Steps s2Step IH=>
+  simp [systemIsValid, ] at (IH)
+  have IHApp := IH s0; simp [s0Inits, s0Steps] at IHApp
+  have s2Valid:(systemIsValid s2) := by (simp [systemIsValid]; grind)
+  --have IH2 := inv43Proof s2 v i id s2Valid
+  exact (inv43Proof_ind s2 s3 i v id s2Step IHApp (idIsK s2 s2Valid))
+
+
+
+theorem inv42Proof_ind (s1 s2: System a l p) (i: Fin a)  (v: Value) (id: PropId) :
+step s1 s2
+-> inv42 s1 i v id
+-> (∀ i, (s1.acceptors i).id = i)
+-> inv43 s1 i v id
+-> inv42 s2 i v id := by
+simp [inv42]; intros step IH kIsTrue i43  learnInN
+cases step <;> rename_i stepRule <;> cases stepRule <;> (try (rename_i stepRule; simp at stepRule; grind)) <;> (try (simp [updateMap] at *; split <;> try grind  ))
+. rename_i j pid mess acc net  stepRule eq;
+  rcases stepRule with ⟨ mRules, accNat, natRules ⟩ 
+  subst_vars; simp; rw [natRules] at learnInN; simp at learnInN
+  have IHApp := IH learnInN
+  exact Nat.le_of_lt (Nat.lt_of_le_of_lt  IHApp mRules.right.right)
+. have IHApp := IH learnInN; rename_i stepRule eq
+  rcases stepRule with ⟨ mNat, idBound, mInN, a2Nat ⟩; subst a2Nat ; simp; subst eq
+  exact (Nat.le_trans  IHApp idBound)
+. rename_i j net v' pid stepRule
+  rcases stepRule with ⟨ accIsSome , netNat ⟩ ; rw [netNat] at learnInN
+  simp at learnInN; cases learnInN <;> try grind
+  rename_i eq; rcases eq with ⟨ eq1, eq2, eq3 ⟩;
+  subst_vars; rw [kIsTrue j] at *
+  simp at *; have bound :=  i43 accIsSome
+  simp [bound]
+  
+
+theorem inv42Proof (s: System a l p) (v: Value) (i: Fin a) (id: PropId)  :
+systemIsValid s
+-> inv42 s i v id:= by
+intros sIsValid
+have ⟨ s0, s0Inits, s0Steps ⟩ := sIsValid
+induction s0Steps  with
+| refl =>
+  simp [systemInits, networkInits] at s0Inits
+  simp [inv42, s0Inits] at ⊢
+| trans s2 s3 s0Steps s2Step IH=>
+  simp [systemIsValid, ] at (IH)
+  have IHApp := IH s0; simp [s0Inits, s0Steps] at IHApp
+  have s2Valid:(systemIsValid s2) := by (simp [systemIsValid]; grind)
+  have IH2 := inv43Proof s2 v i id s2Valid
+  exact (inv42Proof_ind s2 s3 i v id s2Step IHApp (idIsK s2 s2Valid) IH2)
+
+
+
+theorem inv41Proof_ind (s1 s2: System a l p) (i: Fin a)  (v: Value) (id: PropId) :
+step s1 s2
+-> inv41 s1 i v id
+-> (∀ i, (s1.acceptors i).id = i)
+-> inv42 s1 i v id
+-> inv41 s2 i v id := by
+simp [inv41]; intros step IH iBound i42 learnInN
+cases step <;> rename_i stepRule <;> cases stepRule <;> try (rename_i stepRule; simp at stepRule; grind)
+. rename_i j pid mess acc net stepRule
+  simp [updateMap] at *
+  split <;> try grind  
+. rename_i pid j v' acc mess stepRule
+  simp [updateMap] at *
+  split <;> try grind
+  rcases stepRule with ⟨ mNat, mIdBound, mInN, accNat ⟩; subst accNat
+  simp;
+  have dd := i42 learnInN; rename_i eq; subst eq
+  exact (Nat.le_trans dd mIdBound)
+. rename_i j net v' pid stepRule
+  rcases stepRule with ⟨ sAcc, nNat ⟩; simp at learnInN;rw [nNat] at learnInN; simp at ⊢ learnInN
+  cases learnInN <;> try grind
+  rename_i eqs; rcases eqs with ⟨ iId, vEq, idEq ⟩; subst_vars
+  exists v'; exists pid; simp [PropId, iBound]; exact sAcc
+
+theorem inv41Proof (s: System a l p) (v: Value) (i: Fin a) (id: PropId)  :
+systemIsValid s
+-> inv41 s i v id:= by
+intros sIsValid
+have ⟨ s0, s0Inits, s0Steps ⟩ := sIsValid
+induction s0Steps  with
+| refl =>
+  simp [systemInits, networkInits] at s0Inits
+  simp [inv41, s0Inits] at ⊢
+| trans s2 s3 s0Steps s2Step IH=>
+  simp [systemIsValid, ] at (IH)
+  have IHApp := IH s0; simp [s0Inits, s0Steps] at IHApp
+  have s2Valid:(systemIsValid s2) := by (simp [systemIsValid]; grind)
+  have IH2 := inv42Proof s2 v i id s2Valid
+  exact (inv41Proof_ind s2 s3 i v id s2Step IHApp (idIsK s2 s2Valid) IH2)
+
+
+
+
+theorem some_to_learn_ind (s1 s2: System a l p) (v : Value) (j: Fin l) :
+step s1 s2
+-> ((s1.learners j).decide = some v -> ∃ id, learn_invariant s1 v j id)
+-> ((s2.learners j).decide = some v -> ∃ id, learn_invariant s2 v j id)
+:= by
+   intros step IH sLearnDec; simp [learn_invariant] at *
+   cases step <;> rename_i stepRule <;> cases stepRule <;> try (simp at sLearnDec; have ⟨ id, s, rest ⟩ := IH sLearnDec; exists id; exists s; try grind)
+   . rename_i i learn mess v' pid k stepRule; simp at stepRule;
+     rcases stepRule with ⟨ messNat, messInN, l1None, l2Nat ⟩; subst l2Nat
+     simp [updateMap] at sLearnDec ⊢ ; split at sLearnDec
+     . exists pid; grind
+     . have ⟨ pid2, s, rest ⟩  := IH sLearnDec; exists pid2; exists s; grind
+   . rename_i l2 v i pid stepRule
+     rcases stepRule with ⟨ s, sCount, sContains, l1Nat, l2Nat ⟩ ; subst l2Nat
+     simp [updateMap] at sLearnDec ⊢; split at sLearnDec
+     . exists pid; grind
+     . have ⟨ pid2, s, rest ⟩  := IH sLearnDec; exists pid2; exists s; grind
+     
+
+
+theorem some_to_learn_holds (s: System a l p) (v : Value) (j: Fin l) :
+systemIsValid s
+ ->
+ ((s.learners j).decide = some v -> ∃ id, learn_invariant s v j id) := by
+    intros sIsValid sDec
+    rcases sIsValid with ⟨ s0, s0Inits, s0Steps ⟩
+    induction s0Steps with
+    | refl =>
+      simp [systemInits, learnerInits] at s0Inits
+      simp [s0Inits] at sDec
+    | trans s2 s3 s0Steps s2Step IH=>
+      exact (some_to_learn_ind s2 s3 v j s2Step IH sDec)
+
+theorem inv2Proof_ind (s1 s2: System a l p) (j: Fin l) (i: Fin a) (v: Value) (id: PropId) :
+step s1 s2
+-> inv2 s1 j i v id
+-> inv2 s2 j i v id := by
+simp [inv2]; intros step IH sIsSome
+cases step <;> rename_i stepRule <;> cases stepRule <;> try (rename_i stepRule; simp at stepRule; grind)
+. rename_i k l2 m v' pid c stepRule
+  rcases stepRule with ⟨ mIsLearn, mInN, decIsNone, l2Nat⟩; subst l2Nat 
+  simp; simp [updateMap] at sIsSome; split at sIsSome <;> try grind
+  simp [updateMap] at sIsSome <;> split at sIsSome <;> try grind
+. rename_i l2 v k pid stepRule
+  simp [updateMap] at sIsSome; split at sIsSome <;> try grind
+  rcases stepRule with ⟨ set, countSet, setContains, decisNone, l2Nat⟩; subst l2Nat; simp at ⊢ sIsSome
+  grind
+
+theorem inv2Proof (s: System a l p) (j: Fin l) (i: Fin a) (v: Value) (id: PropId) :
+systemIsValid s
+-> inv2 s j i v id := by
+intros sIsValid 
+rcases sIsValid with ⟨ s0, s0Inits, s0Steps ⟩
+induction s0Steps  with
+| refl =>
+  simp [systemInits, learnerInits] at s0Inits
+  simp [inv2, s0Inits] at ⊢ 
+| trans s2 s3 s0Steps s2Step IH=>
+  exact (inv2Proof_ind s2 s3 j i v id s2Step IH)
+  
+
+theorem inv31Proof_ind (s1 s2: System a l p) (i: Fin a) (v: Value) (id: PropId) :
+step s1 s2
+-> inv31 s1 i v id
+-> inv31 s2 i v id := by
+simp [inv31]; intros step  IH accIsSome
+cases step <;> rename_i stepRule <;> cases stepRule <;> try (rename_i stepRule; simp at stepRule; grind)
+. rename_i j pid m acc n stepRule; simp [updateMap] at *
+  split at accIsSome <;> try grind
+. rename_i pid j v' acc m stepRule; simp [updateMap] at *
+  split at accIsSome <;> try grind
+
+
+theorem inv31Proof (s: System a l p) (i: Fin a) (v: Value) (id: PropId) :
+systemIsValid s
+-> inv31 s i v id := by
+intros sIsValid 
+rcases sIsValid with ⟨ s0, s0Inits, s0Steps ⟩
+induction s0Steps  with
+| refl =>
+  simp [systemInits, acceptorInits] at s0Inits
+  simp [inv31, s0Inits] at ⊢ 
+| trans s2 s3 s0Steps s2Step IH=>
+  exact (inv31Proof_ind s2 s3 i v id s2Step IH)
+
+
+
+
+theorem inv3Proof_ind (s1 s2: System a l p) (i: Fin a) (v: Value) (id: PropId) :
+step s1 s2
+-> inv3 s1 i v id
+-> (∀ i, (s1.acceptors i).id = i)
+-> inv31 s1 i v id
+-> inv3 s2 i v id := by
+simp [inv3, inv31]; intros step  IH accIsK IH2 sIsSome
+cases step <;> rename_i stepRule <;> cases stepRule <;> try (rename_i stepRule; simp at stepRule; grind)
+
+
+
+
+theorem inv3Proof (s: System a l p) (i: Fin a) (v: Value) (id: PropId) :
+systemIsValid s
+-> inv3 s i v id := by
+intros sIsValid
+have ⟨ s0, s0Inits, s0Steps ⟩ := sIsValid
+induction s0Steps  with
+| refl =>
+  simp [systemInits, networkInits] at s0Inits
+  simp [inv3, s0Inits] at ⊢ 
+| trans s2 s3 s0Steps s2Step IH=>
+  simp [systemIsValid, ] at (IH)
+  have IHApp := IH s0; simp [s0Inits, s0Steps] at IHApp
+  have s2Valid:(systemIsValid s2) := by (simp [systemIsValid]; grind)
+  have IH2 := inv31Proof s2 i v id s2Valid
+  exact (inv3Proof_ind s2 s3 i v id s2Step IHApp (idIsK s2 s2Valid) IH2)
+
+theorem inv4a1Proof_ind (s1 s2: System a l p) (i: Fin a) (v: Value) (id: PropId) :
+step s1 s2
+-> inv4a1 s1 i v id
+-> inv4a1 s2 i v id := by
+simp [inv4a1]; intros step IH sIsSome
+cases step <;> rename_i stepRule <;> cases stepRule <;> (try (rename_i stepRule; simp at stepRule; grind))
+. rename_i j pid mess acc net stepRule
+  rcases stepRule with ⟨mRules, accNat, netNat⟩; subst accNat
+  simp; rw [netNat]; simp; clear netNat; simp [updateMap] at sIsSome; split at sIsSome <;> try grind  
+. rename_i pid j v' acc mess stepRule
+  simp [updateMap] at ⊢ sIsSome; split at sIsSome <;> try grind
+  rcases stepRule with ⟨ mAcc, accBound, mInN, accNat⟩; subst accNat mAcc
+  simp at sIsSome; rcases sIsSome with ⟨ eq1, eq2 ⟩; subst eq1 eq2
+  exact mInN
+
+theorem inv4cProof_ind (s1 s2: System a l p) (v: Value) (id: PropId) :
+step s1 s2
+-> inv4c s1 v id
+-> inv4c s2 v id := by
+simp [inv4c]; intros step IH sIsSome
+cases step <;> rename_i stepRule <;> cases stepRule <;> (try (rename_i stepRule; simp [updateMap] at *; grind))
+. rename_i j pid mess acc net stepRule
+  rcases stepRule with ⟨ mProp, accNat , netNat ⟩; subst accNat
+  rw [netNat] at sIsSome; simp at sIsSome
+  have ⟨ set, setCount, setContains ⟩ := IH sIsSome; clear IH
+  exists set; simp [setCount, updateMap]
+  cases setContains <;> try grind
+  left; intros i;split
+  rename_i eq d;subst j; simp; exact (eq i)
+  rename_i eq d; exact (eq i)
+  right; sorry
+. rename_i v' net p stepRule
+  rcases stepRule with ⟨ countHave, choice ⟩
+  sorry
+. simp at sIsSome
+  sorry
+
+
+
+theorem inv4cProof (s: System a l p) (v: Value) (id: PropId)  :
+systemIsValid s
+-> inv4c s v id:= by
+intros sIsValid 
+rcases sIsValid with ⟨ s0, s0Inits, s0Steps ⟩
+induction s0Steps  with
+| refl =>
+  simp [systemInits, networkInits] at s0Inits
+  simp [inv4c, s0Inits] at ⊢ 
+| trans s2 s3 s0Steps s2Step IH=>
+  exact (inv4cProof_ind s2 s3 v id s2Step IH)
+
+
+theorem inv4b1Proof (s: System a l p) (v1 v2: Value) (id: PropId)  :
+systemIsValid s
+-> inv4b1 s v1 v2 id:= by 
+sorry
+
+theorem inv4bProof (s: System a l p) (v: Value) (id: PropId)  :
+systemIsValid s
+-> inv4b s v id:= by 
+intros svalid setRule id1 v' mAccs idBound
+rcases setRule with ⟨ set1, set1Count, set1Contains ⟩
+have ⟨ set2, set2Count, setRules⟩  := inv4cProof s v' id1 svalid mAccs
+have cc := setMaxContainsBoth set1 set2 (by simp [set1Count]); simp [set2Count] at cc
+rcases cc with ⟨ i, set1ContainsI, set2ContainsI ⟩
+have p1 := set1Contains i set1ContainsI
+rcases setRules with c1 | c2
+. have p2 : (∀ id2 v', id2 < id1 -> (s.acceptors i).accepted ≠ some (v', id2)) := by {intros id2 v' idBound; grind}
+  
+  
+  
+  
+  
+. sorry
+/-
+induction id1 using Nat.strongRecOn 
+rename_i n IH
+intros setRule v' mAcc iBound
+rcases setRule with ⟨set, setCount, setContains⟩
+have ⟨set2, setCount2, set2Contains1⟩ := inv4cProof s v' n svalid mAcc
+have dd := setMaxContainsBoth set set2 (by simp [setCount])
+simp [setCount2] at dd; rcases dd with  ⟨ i, i1Cont, i2Cont ⟩
+have hLearn := setContains i i1Cont
+have ⟨v'', id'', hge, hAcc⟩ := (inv41Proof s v i id) svalid hLearn
+rcases set2Contains1 with hA | hB
+
+
+. have hAccV := (inv3Proof s i v id) svalid hLearn
+  by_cases hid : (id = n) 
+  · subst hid
+    exact inv4b1Proof s v v' id svalid hAccV mAcc
+  . have ⟨ set3, set3Count, set3Rules ⟩   := inv4cProof s v' n svalid mAcc
+    rcases set3Rules with hLeft | hRight
+    obtain ⟨j, hj1, hj3⟩ := setMaxContainsBoth set set3 setCount set3Count
+    have hjLearn := setContains j hj1
+    have h41 := (inv41Proof s  v j id) svalid hjLearn
+    obtain ⟨vj, idj, hidj, hjAcc⟩ := h41
+    have hno := hLeft j hj3
+    simp  at hno; have contra := hno idj vj hjAcc
+-/
+    
+    
+  
+
+theorem inv4a1Proof (s: System a l p) (i: Fin a) (v: Value) (id: PropId)  :
+systemIsValid s
+-> inv4a1 s i v id:= by 
+intros sIsValid 
+rcases sIsValid with ⟨ s0, s0Inits, s0Steps ⟩
+induction s0Steps  with
+| refl =>
+  simp [systemInits, acceptorInits] at s0Inits
+  simp [inv4a1, s0Inits] at ⊢ 
+| trans s2 s3 s0Steps s2Step IH=>
+  exact (inv4a1Proof_ind s2 s3 i v id s2Step IH)
+
+
+
+
+theorem inv4aProof (s: System a l p) (v: Value) (id: PropId)  :
+systemIsValid s
+-> inv4a s v id:= by
+intros sIsValid set id1 i v' accIn idBound
+have p2 := inv4a1Proof s i v' id1 sIsValid accIn
+exact (inv4bProof s v id sIsValid set id1 v' p2 idBound)
+
+
+theorem inv4Proof (s: System a l p) (v: Value) (id: PropId) :
+systemIsValid s
+-> inv4 s v id := by
+intros svalid IH
+have ⟨ set, countSet, setContains ⟩ := IH
+have p1 := inv41Proof s v
+have p2 := inv4aProof s v id svalid  IH
+have ⟨ set2, set2Count, set2Contains ⟩ : (∃ (set : Set a), count set > a / 2 ∧
+    (∀ i, contains set i →
+      ∃ id' v', id' >= id ∧ (s.acceptors i).accepted = some (v', id'))) := by {
+      exists set; simp [countSet]; intro i containsI
+      have ⟨ v, id1, id1Bound, sAcc ⟩ := p1 i id svalid (setContains i containsI); exists id1; simp [id1Bound]; exists v 
+}
+have set2Contains_ :(∀ (i : Fin a), contains set2 i = true → ∃ id', id' ≥ id ∧ (s.acceptors i).accepted = some (v, id')) := by {
+intros i containsI; have ⟨ id', v', idBound ⟩ := set2Contains i containsI
+exists id'; simp [idBound]; rw [p2 id' i v' idBound.right idBound.left]
+}
+simp [acc_invariant]
+exists id; simp [PropId]
+exists set2
+
+
+
+theorem ind_proof (s: System a l p) (v: Value) (i: Fin l) :
+systemIsValid s
+-> (s.learners i).decide = some v
+-> ∃ id, acc_invariant s v id := by
+   intros svalid sDevSome
+   have ⟨ id, p1 ⟩  := some_to_learn_holds s v i svalid sDevSome;
+   rcases p1 with ⟨ set, setCount, setContains⟩ 
+   simp [acc_invariant]; 
+   have cc : (∃ set, count set > a / 2 ∧ (∀ (i: Fin a), contains  set i -> Message.Learn (i, v, id) ∈ s.network.messages)) := by exists set; simp [setCount]; intros j contj; have cc := setContains j contj; exact inv2Proof s i j v id svalid cc
+   have  ⟨  id', id'Bound, rest ⟩  := inv4Proof s v id svalid cc; exists id'
+   
+
+theorem acc_eqs (s1: System a l p) (v1 v2: Value) (id: PropId) (id': PropId):
+acc_invariant s1 v1 id 
+-> acc_invariant s1 v2 id'
+-> v1 = v2 := by 
+   intros acc1 acc2; simp [acc_invariant] at acc1 acc2
+   rcases acc1 with ⟨ set1, set1Counts, set1Contains ⟩
+   rcases acc2 with ⟨ set2, set2Counts, set2Contains ⟩ 
+   have ⟨ i, contain1, contain2 ⟩ := setMaxContainsBoth set1 set2 set1Counts set2Counts
+   have ⟨ id1, accSome1 ⟩  := set1Contains i contain1
+   
+   have ⟨ id2, accSome2 ⟩  := set2Contains i contain2; simp [accSome2] at accSome1 ; simp [accSome1]
+
+
+
+theorem learners_choice_is_unique (s : System a l p):
+ ∀ i j v1 v2, systemIsValid s -> (s.learners i).decide = some v1 -> (s.learners j).decide = some v2 -> v1 = v2 := by
+  intros i j v1 v2 sIsValid sDecSome1 sDecSome2
+  have ⟨ id1, t1⟩  := ind_proof s v1 i sIsValid sDecSome1
+  have ⟨ id2, t2 ⟩  := ind_proof s v2 j sIsValid sDecSome2
+  exact (acc_eqs s v1 v2 id1 id2 t1 t2) 
+  
